iso_dh/initiator.v
@@ -43,32 +43,31 @@ Definition initiator : val := λ: "c" "skI" "vkR",
 Ltac protocol_failure :=
   by intros; wp_pures; iApply ("Hpost" $! None); iFrame.
 
-Lemma wp_initiator c kI kR :
+Lemma wp_initiator c skI vkR :
   channel c -∗
   cryptis_ctx -∗
   iso_dh_ctx N -∗
-  public (TKey Open kI) -∗
-  public (TKey Open kR) -∗
+  sign_key skI -∗
+  public vkR -∗
   {{{ True }}}
-    initiator c kI (TKey Open kR)
+    initiator c skI vkR
   {{{ okS, RET (repr okS);
       if okS is Some kS then ∃ si failed,
-        ⌜si_init si = kI⌝ ∗
-        ⌜si_resp si = kR⌝ ∗
+        ⌜si_init si = skI⌝ ∗
+        ⌜TKey Open (si_resp si) = vkR⌝ ∗
         ⌜si_key si = kS⌝ ∗
         minted kS ∗
         session_status si failed ∗
-        □ (∀ kt, public (TKey kt kS) ↔ ◇ public kS) ∗
+        senc_key kS ∗
         □ (◇ public kS ↔ ▷ ⌜failed⌝) ∗
-        (compromised si ∨ ⌜failed = false⌝) ∗
+        (compromised_session si ∨ ⌜failed = false⌝) ∗
         term_token (si_init_share si) ⊤
       else True
  }}}.
 Proof.
 rewrite /initiator.
-set vkI := TKey Open kI.
-set vkR := TKey Open kR.
-iIntros "#chan_c #ctx #(? & ?) #p_kI #p_kR %Ψ !> phase Hpost".
+set vkI := TKey Open skI.
+iIntros "#chan_c #ctx #(? & ?) #skI #p_vkR %Ψ !> _ Hpost".
 wp_pures. wp_apply wp_vkey. wp_pures. rewrite -/vkI.
 wp_apply (wp_mknonce_freshN ∅
             (λ a, term_meta a (nroot.@"failed") true)
@@ -97,56 +96,51 @@ iAssert (public ga) as "p_ga".
   iApply "a_pred". iModIntro. iModIntro.
   by rewrite /iso_dh_pred exps_TExpN. }
 wp_apply wp_send => //.
-{ rewrite public_of_list /=. do 2?[iSplit => //]. }
+{ rewrite public_of_list /=. do 2?[iSplit => //].
+  by iApply sign_key_public. }
 wp_pure _ credit:"H3".
 wp_pures. wp_apply wp_recv => //.
 iIntros "%m2 #p_m2".
-wp_verify m2; last by protocol_failure.
+wp_apply wp_verify.
+case: Spec.decP; last by protocol_failure.
+move=> skR {}m2 -> -> {vkR}. set vkR := TKey Open skR.
 wp_pures. wp_list_of_term m2; last by protocol_failure.
 wp_pures. wp_list_match => [ga' gb vkI' -> {m2}|]; last by protocol_failure.
 wp_eq_term e; last by protocol_failure. subst ga'.
 wp_pures. wp_eq_term e; last by protocol_failure. subst vkI'.
-iAssert (public gb)%I as "#p_gb".
-{ iPoseProof (public_TSealE with "p_m2 [//]") as "[p|p]".
-  - rewrite public_of_list /=.
-    by iDestruct "p" as "(_ & _ & ? & _)".
-  - iDestruct "p" as "(_ & _ & #p)".
-    iSpecialize ("p" with "p_kR").
-    rewrite public_of_list /=.
-    by iDestruct "p" as "(_ & ? & ? & _)". }
-iPoseProof (public_minted with "p_m2") as "m_m2".
-rewrite minted_TSeal minted_tag minted_of_list /=.
-iDestruct "m_m2" as "(_ & _ & m_gb & _)".
+iPoseProof (public_signE with "p_m2 [//] [//]") as "{p_m2} [p_m2 inv]".
+rewrite public_of_list /=. iDestruct "p_m2" as "(_ & p_gb & _)".
+iPoseProof (public_minted with "p_gb") as "m_gb".
 wp_pures. wp_bind (texp _ _). iApply wp_texp.
 wp_pures. wp_list. wp_term_of_list. wp_pures.
 set gab := TExp gb a.
 set seed := Spec.of_list [vkI; vkR; ga; gb; gab].
 set secret := Spec.derive_key seed.
 wp_pures. wp_list. wp_term_of_list. wp_apply wp_sign. wp_pures.
-pose si := SessInfo kI kR ga gb gab.
+pose si := SessInfo skI skR ga gb gab.
 iAssert (|={⊤}=> ∃ failed,
   session_status si failed ∗
   □ (◇ public (si_key si) ↔ ▷ ⌜failed⌝) ∗
-  (compromised si ∨ ⌜failed = false⌝))%I
+  (compromised_session si ∨ ⌜failed = false⌝))%I
   with "[token_a H3]"
-  as "{p_m2} > (%failed & #status & #s_key & #p_skR)".
-{ iPoseProof (public_TSealE with "p_m2 [//]") as "{p_m2} p_m2".
-  iDestruct "p_m2" as "[[comp _]  | (#i_m2 & _ & _)]".
+  as "{inv} > (%failed & #status & #s_key & #p_skR)".
+{ iDestruct "inv" as "[comp|#inv]".
   { iMod (term_meta_set (nroot.@"failed") true with "token_a")
       as "#failed" => //.
-    iModIntro. iExists true. rewrite /session_status /compromised.
+    iModIntro. iExists true. rewrite /session_status /compromised_session.
     iSplit; first by eauto.
-    iSplit; last by eauto.
+    iSplit; last by iLeft; iRight.
     iModIntro.
     iSplit; iIntros "_" => //.
     iIntros "!>". rewrite public_derive_key public_of_list /=.
     do !iSplit => //.
+    { by iApply sign_key_public. }
     iApply public_TExp => //.
     by iApply "s_a". }
-  iMod (lc_fupd_elim_later_pers with "H3 i_m2") as "{i_m2} #i_m2".
+  iMod (lc_fupd_elim_later_pers with "H3 inv") as "{inv} #inv".
   iMod (term_meta_set (nroot.@"failed") false with "token_a")
     as "#failed" => //.
-  iDestruct "i_m2" as "(%ga' & %b & %kI' & %e_m2 & s_b & pred_b)".
+  iDestruct "inv" as "(%ga' & %b & %kI' & %e_m2 & s_b & pred_b)".
   iAssert (public a ↔ ▷ □ False)%I as "{s_a} s_a".
   { iApply (bi.iff_trans _ (▷ □ term_meta a (nroot.@"failed") true)).
     iSplit => //.
@@ -162,23 +156,19 @@ iAssert (|={⊤}=> ∃ failed,
   iApply (bi.iff_trans _ (◇ public gab)).
   iSplit; last by iApply public_dh_secret.
   rewrite public_derive_key public_of_list /=.
-  iSplit; last by iIntros "#?"; do !iSplit.
-  by iIntros ">(_ & _ & _ & _ & ? & _)". }
+  iSplit; first by iIntros ">(_ & _ & _ & _ & ? & _)".
+  iIntros ">#?"; do !iSplit => //. iModIntro. by iApply sign_key_public. }
 set m3 := Spec.enc _ _ _.
 iAssert (public m3) as "#p_m3".
-{ iApply (public_TSealIS with "[] [//] [#]") => //.
-  - by rewrite !public_minted !minted_TKey.
-  - iExists a, gb, kR, failed. by do 3![iSplitR => //].
-  - rewrite minted_of_list /= minted_TExp /= minted_TInt minted_TKey.
-    rewrite !public_minted !minted_TKey. by do ![iSplitL => //].
-  - iIntros "!> _".
-    rewrite public_of_list /=.
-    by do ![iSplit => //]. }
+{ iApply (public_signIS with "[] [//] [#]") => //.
+  - iExists a, gb, skR, failed. by do 3![iSplitR => //].
+  - rewrite public_of_list /=. by do ![iSplit => //]. }
 wp_pures. wp_apply wp_send => //.
 wp_pures. wp_apply wp_derive_key.
 iAssert (minted seed) as "#m_seed".
 { rewrite minted_of_list /= !minted_TExp /= minted_TInt.
-  by do !iSplit => //; iApply public_minted. }
+  do !iSplit => //; iApply public_minted => //.
+  by iApply sign_key_public. }
 wp_pures. iApply ("Hpost" $! (Some secret)).
 iExists si, failed. iFrame. do !iSplitR => //.
   by rewrite minted_derive_key.
