store/game.v
@@ -50,8 +50,8 @@ Definition game : val := λ: <>,
   (* Connect client to server and leak long-term secret keys after
      connection is done *)
   let: "conn" := Client.connect kvsN "c" "skI" "vkR" in
-  send "c" (key Seal "skI");;
-  send "c" (key Seal "skR");;
+  send "c" "skI";;
+  send "c" "skR";;
 
   (* Store value in server *)
   let: "k" := recv "c" in
@@ -77,7 +77,7 @@ Qed.
 
 Lemma wp_start_server c skR :
   {{{ cryptis_ctx ∗ channel c ∗ store_ctx kvsN ∗
-      public (TKey Open skR) ∗
+      sign_key skR ∗
       term_token skR ⊤ }}}
     start_server c skR
   {{{ RET #(); True }}}.
@@ -98,9 +98,9 @@ iIntros "#ctx enc_tok"; rewrite /game; wp_pures.
 iMod (store_ctx_alloc (N := kvsN) with "enc_tok") as "[#? _]" => //.
 wp_apply wp_init_network => //. iIntros "%c #cP". wp_pures.
 wp_apply (wp_mksigkey with "[]"); eauto.
-iIntros "%skI #p_vkI s_skI tokenI". wp_pures.
+iIntros "%skI #p_vkI #sign_skI s_skI tokenI". wp_pures.
 wp_pures. wp_apply (wp_mksigkey with "[]"); eauto.
-iIntros "%skR #p_vkR s_skR tokenR". wp_pures.
+iIntros "%skR #p_vkR #sign_skR s_skR tokenR". wp_pures.
 wp_apply wp_vkey. wp_pures.
 wp_apply wp_vkey. wp_pures.
 wp_apply wp_send => //. wp_pures.
@@ -114,14 +114,18 @@ wp_apply (wp_client_connect with "[] [] [] [] [] client"); eauto.
 iIntros "%cs client". wp_pure _ credit:"c". wp_pures.
 iCombine "s_skI s_skR" as "s_sk".
 iMod (client_connected_ok with "client s_sk []") as "(s_sk & client & #ok)".
-{ iIntros "[(s_skI & s_skR) [fail|fail]]".
-  - iDestruct (secret_not_public with "s_skI fail") as ">[]".
-  - iDestruct (secret_not_public with "s_skR fail") as ">[]". }
+{ iIntros "[(s_skI & s_skR) #[fail|fail]]".
+  - iPoseProof (sign_key_compromised_keyE with "sign_skI [//]")
+      as ">contra".
+    by iDestruct (secret_not_public with "s_skI contra") as ">[]".
+  - iPoseProof (sign_key_compromised_keyE with "sign_skR [//]")
+      as ">contra".
+  - by iDestruct (secret_not_public with "s_skR contra") as ">[]". }
 iDestruct "s_sk" as "[s_skI s_skR]".
-iMod (compromise_secret with "s_skI") as "#p_skI".
-iMod (compromise_secret with "s_skR") as "#p_skR".
-wp_apply wp_key. wp_apply wp_send => //. wp_pures.
-wp_apply wp_key. wp_apply wp_send => //. wp_pures.
+iMod (secret_public with "s_skI") as "#p_skI".
+iMod (secret_public with "s_skR") as "#p_skR".
+wp_apply wp_send => //. wp_pures.
+wp_apply wp_send => //. wp_pures.
 wp_apply wp_recv => //. iIntros "%k #p_k". wp_pures.
 wp_apply wp_recv => //. iIntros "%v #p_v". wp_pures.
 rewrite (@rem_free_at_diff _ _ _ _ _ _ {[k]}) //.
